src/Lustre/Normalization/Correctness.v
@@ -41,41 +41,39 @@ Module Type CORRECTNESS
       replace (length a) with (length (List.map fst a)) by (rewrite map_length; reflexivity).
       rewrite <- H9. unfold typesof; rewrite flat_map_concat_map.
       apply concat_length_eq.
+      rewrite Forall2_map_2.
       rewrite_Forall_forall; solve_length.
-      erewrite map_nth'; solve_length. rewrite length_typeof_numstreams.
-      eapply H0...
+      rewrite length_typeof_numstreams. eapply H0...
       + apply nth_In; congruence.
       + apply H5. apply nth_In; congruence.
     - (* when *)
       repeat rewrite_Forall_forall.
       rewrite <- H1. unfold typesof; rewrite flat_map_concat_map.
       apply concat_length_eq.
+      rewrite Forall2_map_2.
       rewrite_Forall_forall; solve_length.
-      erewrite map_nth'. rewrite length_typeof_numstreams.
-      eapply H0...
+      rewrite length_typeof_numstreams. eapply H0...
       + apply nth_In; congruence.
       + apply H5. apply nth_In; congruence.
-      + congruence.
     - (* merge *)
       repeat rewrite_Forall_forall.
       rewrite <- H11. unfold typesof; rewrite flat_map_concat_map.
       apply concat_length_eq.
+      rewrite Forall2_map_2.
       rewrite_Forall_forall; solve_length.
-      erewrite map_nth'. rewrite length_typeof_numstreams.
-      eapply H0...
+      rewrite length_typeof_numstreams. eapply H0...
       + apply nth_In; congruence.
       + apply H6. apply nth_In; congruence.
-      + congruence.
     - (* ite *)
       repeat rewrite_Forall_forall.
       rewrite <- H12. unfold typesof; rewrite flat_map_concat_map.
       apply concat_length_eq.
+      rewrite Forall2_map_2.
       rewrite_Forall_forall; solve_length.
-      erewrite map_nth'. rewrite length_typeof_numstreams.
+      rewrite length_typeof_numstreams.
       eapply H0...
       + apply nth_In; congruence.
       + apply H7. apply nth_In; congruence.
-      + congruence.
     - (* app *)
       destruct H11.
       rewrite H3 in H6; clear H3; inv H6.
@@ -88,10 +86,28 @@ Module Type CORRECTNESS
       repeat rewrite_Forall_forall.
       unfold idents in H5.
       solve_length.
-      Unshelve. 1,2,3,4:exact (hd_default []).
   Qed.
 
-  Corollary normalize_exp_sem_length : forall G vars e is_control es' eqs' st st',
+  Corollary sem_exps_numstreams : forall G vars H b es vs,
+      Forall (wt_exp G vars) es ->
+      Forall2 (sem_exp G H b) es vs ->
+      length (concat vs) = length (annots es).
+  Proof.
+    intros G vars H b es vs Hwt Hsem.
+    assert (Forall2 (fun v e => length v = numstreams e) vs es) as Hf.
+    { repeat rewrite_Forall_forall.
+      eapply sem_exp_numstreams.
+      + eapply Hwt. eapply nth_In. solve_length.
+      + eapply H1; eauto. solve_length. }
+    clear Hwt Hsem.
+    induction Hf; simpl.
+    - reflexivity.
+    - repeat rewrite app_length.
+      f_equal; auto.
+      rewrite length_annot_numstreams. assumption.
+  Qed.
+
+  Fact normalize_exp_sem_length : forall G vars e is_control es' eqs' st st',
       wt_exp G vars e ->
       normalize_exp is_control e st = (es', eqs', st') ->
       Forall (fun e => forall v H b,
@@ -146,16 +162,16 @@ Module Type CORRECTNESS
   Qed.
 
   Hint Constructors sem_exp.
-  Fact normalize_exp_sem : forall G vars b e H v is_control es' eqs' st st',
+  Fact normalize_exp_sem : forall G vars b e H vs is_control es' eqs' st st',
       wt_exp G vars e ->
-      sem_exp G H b e v ->
+      sem_exp G H b e vs ->
       normalize_exp is_control e st = (es', eqs', st') ->
       (exists H',
           Env.refines eq H H' /\
-          Forall2 (fun e v => sem_exp G H' b e [v]) es' v /\
+          Forall2 (fun e v => sem_exp G H' b e [v]) es' vs /\
           Forall (sem_equation G H' b) eqs').
   Proof with eauto.
-    induction e using exp_ind2; intros Hi v is_control es' eqs' st st' Hwt Hsem Hnorm;
+    induction e using exp_ind2; intros Hi vs is_control es' eqs' st st' Hwt Hsem Hnorm;
       inv Hwt; inv Hsem; simpl in Hnorm; repeat inv_bind.
     - (* const *)
       exists Hi. repeat split...
@@ -199,21 +215,71 @@ Module Type CORRECTNESS
     - (* when *)
       specialize (map_bind2_normalize_exp_length _ _ _ _ _ _ _ _ H4 H0) as Hlength.
       erewrite <- (map_length _ (annots es)) in Hlength. erewrite <- typesof_annots in Hlength.
-      eapply map_bind2_sem in H0...
-      + destruct H0 as [H' [Href [Hsem1 Hsem2]]].
-        apply Forall2_concat in Hsem1.
-        exists H'. repeat split; simpl...
-        repeat rewrite_Forall_forall; simpl; solve_length.
-        repeat Typ.simpl_nth. Unshelve. 2: exact (hd_default [], Op.bool_type).
-        destruct (nth n _) eqn:Hnth. Typ.simpl_nth.
-        econstructor.
-        * repeat constructor.
-          eapply H1...
-        * eapply sem_var_refines; eauto.
-        * simpl. repeat constructor.
-          eapply H3...
-      + repeat rewrite_Forall_forall.
-        eapply nth_In in H8...
+      eapply map_bind2_sem in H0... 2: (repeat rewrite_Forall_forall; eapply nth_In in H8; eauto).
+      destruct H0 as [H' [Href [Hsem1 Hsem2]]].
+      apply Forall2_concat in Hsem1.
+      exists H'. repeat split; simpl...
+      rewrite Forall2_map_1.
+      eapply Forall2_trans_ex in H13; [| eauto].
+      apply Forall2_combine_lr with (zs:=(typesof es)) in H13; auto.
+      eapply Forall2_impl_In; [| eauto].
+      intros; simpl in H2. destruct a. destruct H2 as [y [Hin [Hsem Hsem']]].
+      econstructor...
+      + eapply sem_var_refines...
+      + simpl. repeat constructor...
+    - (* merge *)
+      (* specialize (map_bind2_normalize_exp_length _ _ _ _ _ _ _ _ H5 H1) as Hlength1. *)
+      (* specialize (map_bind2_normalize_exp_length _ _ _ _ _ _ _ _ H6 H2) as Hlength2. *)
+      specialize (sem_exps_numstreams _ _ _ _ _ _ H5 H15) as Hlength3.
+      eapply map_bind2_sem in H1... 2:(repeat rewrite_Forall_forall; eapply nth_In in H17; eauto).
+      destruct H1 as [H' [Href1 [Hsem1 Hsem1']]]. apply Forall2_concat in Hsem1.
+      assert (Forall2 (sem_exp G H' b) efs fs) as Hsem' by (repeat rewrite_Forall_forall; eapply sem_exp_refines; eauto).
+      clear H16.
+      eapply map_bind2_sem in H2... 2:(repeat rewrite_Forall_forall; eapply nth_In in H18; eauto).
+      destruct H2 as [H'' [Href2 [Hsem2 Hsem2']]]. apply Forall2_concat in Hsem2.
+      destruct is_control; repeat inv_bind.
+      + (* control *)
+        exists H''. repeat split; simpl...
+        * etransitivity...
+        * rewrite Forall2_map_1.
+          repeat rewrite typesof_annots in H9.
+          assert (length (annots efs) = length (annots ets)) as Hlena by (erewrite <- map_length; erewrite H9; solve_length).
+          repeat rewrite_Forall_forall; solve_length.
+          destruct (nth n (combine _ _) _) as [[? ?] ?] eqn:Hnth.
+          destruct a as [[de de0] dt]. repeat simpl_nth.
+          econstructor.
+          -- apply sem_var_refines with (H:=Hi)... etransitivity...
+          -- repeat econstructor.
+             eapply sem_exp_refines...
+          -- repeat econstructor...
+          -- repeat econstructor...
+        * rewrite Forall_app. split; auto.
+          solve_forall. eapply sem_equation_refines...
+          Unshelve. exact default_ann. 1,2:exact b0.
+      + (* exp *)
+        specialize (idents_for_anns_length _ _ _ _ H1) as Hlength.
+        remember (Env.adds (List.map fst x0) vs H'') as H'''. (* dom H (base ++ st') *)
+        assert (Env.refines eq H'' H''') as Href3 by admit. (* Hum... *)
+        exists H'''. repeat split...
+        * repeat (etransitivity; eauto).
+        * rewrite Forall2_map_1.
+          repeat rewrite_Forall_forall; solve_length.
+          destruct (nth _ x0 _) eqn:Hnth.
+          repeat constructor. econstructor; [| reflexivity]. admit. (* More reasoning on adds *)
+        * repeat rewrite Forall_app. repeat split.
+          -- repeat rewrite_Forall_forall. destruct x1 as [xs es].
+             repeat simpl_nth.
+             Unshelve. 2,6: exact (hd_default []). 3,4: exact (xH, default_ann).
+             2,3: exact (hd_default [], hd_default [], Op.bool_type).
+             destruct (nth x1 x0 _) eqn:Hnth1.
+             destruct (nth x1 (combine _ _) _) as [[? ?] ?] eqn:Hnth2; subst.
+             repeat simpl_nth.
+             econstructor.
+             ++ repeat constructor. econstructor; admit.
+             ++ admit.
+          -- solve_forall. repeat (eapply sem_equation_refines; eauto).
+          -- solve_forall. eapply sem_equation_refines...
+        (* ajouter v dans l'environement, appairé avec les variables de x0 *)
   Admitted.
 
   (** ** Conservation of sem_equation *)
@@ -246,14 +312,14 @@ Module Type CORRECTNESS
         solve_forall. eapply sem_equation_refines...
   Qed.
 
-  Lemma normalize_node_sem : forall f n G Hwt ins outs to_cut f' n',
-      find_node f G = Some n ->
-      sem_node G f ins outs ->
-      normalize_node to_cut n (ex_intro _ G Hwt) = n' ->
-      find_node f' G = Some n' ->
-      sem_node G f' ins outs.
+  Lemma normalize_node_sem : forall f n G ins outs to_cut f' n',
+      find_node f (proj1_sig G) = Some n ->
+      sem_node (proj1_sig G) f ins outs ->
+      normalize_node to_cut n G = n' ->
+      find_node f' (proj1_sig G) = Some n' ->
+      sem_node (proj1_sig G) f' ins outs.
   Proof with eauto.
-    intros f n G Hwt ins outs to_cut n' f' Hfind Hsem Hnorm Hfind'; simpl in *.
+    intros f n [G Hwt] ins outs to_cut n' f' Hfind Hsem Hnorm Hfind'; simpl in *.
     inv Hsem. rewrite Hfind in H0. inv H0.
     destruct Hwt as [? [? [? Hwt]]].
     remember (normalize_equations (PS.union to_cut (ps_from_list (List.map fst (n_out n0))))
